basic.v
@@ -1,3 +1,5 @@
+Require Import List.
+Import ListNotations.
 Generalizable All Variables.
 Set Implicit Arguments.
 (* useful tactics for the development *)
@@ -7,6 +9,45 @@ Ltac split_refl2 eq_dec a a' := let H:= fresh in
 Ltac bad_eq := match goal with [Hbad : ?a <> ?a |- _] => contradict Hbad; auto end.
 Ltac inject_pair := match goal with [H: (?a, ?b) = (?c, ?d) |- _] => injection H; intros; subst end.
 Ltac inverts H := inversion H; subst.
+Ltac injects H := injection H; intros; subst.
+Ltac disc := discriminate
+           || (match goal with
+                   [H : (?a :: ?b) = [] |- _] => (destruct a; discriminate H)
+                 | [H : ?a ++ [?b] = [] |- _] => (destruct a; discriminate H)
+                 | [H : [] = (?a :: ?b) |- _] => (destruct a; discriminate H)
+                 | [H : [] = ?a ++ [?b] |- _] => (destruct a; discriminate H)
+                 | [H : [] = (?a ++ ?b) ++ [?c] |- _] => (destruct a,b; discriminate H)
+                 | [H : (?a ++ ?b) ++ [?c] = [] |- _] => (destruct a,b; discriminate H)
+               end).
+Ltac listac := repeat progress (disc || 
+                                     (autorewrite with list in *;
+                                 match goal with
+                                     [H : ?l ++ [?a] = ?r ++ [?b] |- _] =>
+                                     apply app_inj_tail in H; destruct H; try subst
+                                  | [H : ?l ++ [?a] = ?b :: ?r ++ [?c] |- _] =>
+                                    let F := fresh in
+                                    let F' := fresh in
+                                    pose (F := @app_assoc _ [b] r [c]);
+                                     cut ([b] ++ r ++ [c] = (b::r)++[c]);
+                                     [intro F'; rewrite F' in F; rewrite F in H; clear F F'
+                                     |reflexivity]
+                                  | [H : ?a :: ?l ++ [?b] = ?r ++ [?c] |- _] =>
+                                    let F := fresh in
+                                    let F' := fresh in
+                                    pose (F := @app_assoc _ [a] l [b]);
+                                     cut ([a] ++ l ++ [b] = (a::l)++[b]);
+                                     [intro F'; rewrite F' in F; rewrite F in H; clear F F'
+                                     |reflexivity]
+                                  | [H : ?l ++ [?a; ?b] = ?r ++ [?c] |- _] =>
+                                    let F := fresh in
+                                    pose (F := @app_assoc _ l [a] [b]);
+                                     simpl in F; rewrite F in H; clear F
+                                  | [H : ?l ++ [?a] = ?r ++ [?b;?c] |- _] =>
+                                    let F := fresh in
+                                    pose (F := @app_assoc _ r [b] [c]);
+                                     simpl in F; rewrite F in H; clear F
+                                  | [H : In ?a [] |- _] => destruct H
+                                 end)).
 
 Notation "'dec_type' T" := (forall x y : T, {x=y}+{x<>y}) (at level 70, no associativity).
 
