pdcfa.v
@@ -1,0 +1,1127 @@
+Require Vectors.Vector.
+Require Import List ListSet Relation_Definitions Relation_Operators Lexicographic_Product.
+Require Import basic finite reduction balance ListSetFacts.
+
+Import ListNotations.
+Generalizable All Variables.
+Set Implicit Arguments.
+
+Coercion bool_prop := (fun b => b = true).
+
+Section Pushdown.
+Variables (Q Γ : Type).
+
+Inductive PDS : Type :=
+  pds_intro : forall (isQ : Q -> bool) (isΓ : Γ -> bool)
+                     (δ : action_relation Q (Stack_Action Γ))
+                     (ε_within_bounds : forall q q', δ q (eps_action Γ) q' -> (isQ q) /\ (isQ q'))
+                     (push_within_bounds :
+                        forall q γ q', δ q (push_action γ) q' -> (isQ q) /\ (isΓ γ) /\ (isQ q'))
+                     (pop_within_bounds :
+                        forall q γ q', δ q (pop_action γ) q' -> (isQ q) /\ (isΓ γ) /\ (isQ q')),
+                PDS.
+
+Definition pds_rel (pds : PDS) : action_relation Q (Stack_Action Γ) :=
+  match pds with pds_intro _ _ δ _ _ _ => δ end.
+Definition pds_Q (pds : PDS) : Q -> bool :=
+  match pds with pds_intro isQ _ _ _ _ _=> isQ end.
+Definition pds_Γ (pds : PDS) : Γ -> bool :=
+  match pds with pds_intro _ isΓ _ _ _ _ => isΓ end.
+
+Inductive RPDS : Type :=
+  rpds_intro : forall (pds : PDS) (q0 : Q), pds_Q pds q0 -> RPDS.
+
+Definition rpds_pds (rpds : RPDS) := match rpds with rpds_intro pds _ _ => pds end.
+Definition rpds_rel (rpds : RPDS) := (pds_rel (rpds_pds rpds)).
+Definition rpds_Q (rpds : RPDS) := (pds_Q (rpds_pds rpds)).
+Definition rpds_root (rpds : RPDS) := match rpds with rpds_intro _ q0 _ => q0 end.
+Inductive PDS_step (pds : PDS) : (Q * list Γ) -> (Q * list Γ) -> Prop :=
+  eps_trans : forall q q' κ, (pds_rel pds) q (eps_action Γ) q' -> PDS_step pds (q,κ) (q',κ)
+| push_trans : forall q q' γ κ, (pds_rel pds) q (push_action γ) q' -> PDS_step pds (q,κ) (q',γ::κ)
+| pop_trans : forall q q' γ κ, (pds_rel pds) q (pop_action γ) q' -> PDS_step pds (q,γ::κ) (q',κ).
+
+Inductive PDS_legal_step (pds : PDS) : (Q * list Γ) -> (Stack_Action Γ) -> Q -> Prop :=
+  eps_ltrans : forall q q' κ, (pds_rel pds) q (eps_action Γ) q' -> PDS_legal_step pds (q,κ) (eps_action Γ) q'
+| push_ltrans : forall q q' γ κ, (pds_rel pds) q (push_action γ) q' -> PDS_legal_step pds (q,κ) (push_action γ) q'
+| pop_ltrans : forall q q' γ κ, (pds_rel pds) q (pop_action γ) q' -> PDS_legal_step pds (q,γ::κ) (pop_action γ) q'.
+
+Hint Constructors PDS_legal_step PDS_step.
+
+
+(*
+Inductive Balanced_actions (A : Type) : list (Stack_Action A) -> list A -> Prop :=
+  balance_eps : forall las ras res, Balanced_actions (las ++ ras) res ->
+                                    Balanced_actions (las ++ (eps_action A :: ras)) res
+| balance_pushpop : forall las ras γ res,
+                      Balanced_actions (las ++ ras) res ->
+                      Balanced_actions (las ++ [push_action γ; pop_action γ] ++ ras) res
+| balance_empty : Balanced_actions [] []
+| balance_push : forall actions γ res,
+                   Balanced_actions actions res ->
+                   Balanced_actions (actions ++ [push_action γ]) (γ :: res).
+*)
+
+(*
+Lemma remove_actions : forall pds q q',
+                       (exists actions, clos_refl_trans_action_with_actions (pds_rel pds) q actions q')
+                       <-> clos_refl_trans_action (pds_rel pds) q q'.
+Proof.
+  intros; split; [intro actpath; induction actpath|intro path; induction path].
+*)
+
+(*
+(* this doesn't necessarily maintain trace structure, since dcrt is opaque *)
+Lemma action_path_and_none : forall pds (qκ qκ' : Q * list Γ),
+                               direct_clos_refl_trans (PDS_step pds) qκ qκ' <->
+                               exists actions,
+                                 clos_refl_trans_action_with_actions (pds_rel pds) (@PDS_Allow Γ) (fst qκ) actions (fst qκ') /\
+                                 Balance_to_kont ((kont_to_actions (snd qκ)) ++ actions) (snd qκ').
+Proof.
+  intros; split; [intro Hpath|intros [actions [path Hbalanced]]].
+  induction Hpath as [|[q κ] [q' κ'] [q'' κ''] Htrace IH Hstep].
+  exists []; autorewrite with list; auto.
+  destruct IH as [actions [IHtrace [IHactions [IHbalance IHformκ]]]].
+  inversion Hstep as [? ? ? Hred| ? ? ? ? Hred|? ? ? ? Hred]; subst; simpl in *.
+
+  exists (actions ++ [eps_action Γ]); split;
+  [eapply (@rtaa_step _ _ _ _ _ _ _ actions _ _ Hred)
+  |exists IHactions; split;
+   [rewrite app_assoc; unfold Balanced_actions; eapply (drt_append _ IHbalance)
+   |]]; auto.
+
+  exists (actions ++ [push_action γ]); split;
+  [eapply (@rtaa_step _ _ _ _ _ _ _ actions _ _ Hred)
+  |exists (IHactions ++ [push_action γ]); split;
+   [rewrite app_assoc; unfold Balanced_actions; apply balance_actions_at_end
+   |constructor]]; auto.
+
+  exists (actions ++ [pop_action γ]); split;
+  [inversion IHformκ as [|actions' ? ? Hactions]; subst; eapply (@rtaa_step _ _ _ _ _ _ _ actions _ _ Hred)
+  |inversion IHformκ as [|actions' ? ? Hactions]; subst;
+   exists actions'; split;
+   [apply balance_actions_at_end with (actions'' := [pop_action γ]) in IHbalance;
+     do 2 rewrite <- app_assoc in IHbalance; simpl in IHbalance;
+     eapply (drt_append IHbalance);
+     eapply drt_step;[apply drt_refl
+                     |set (H:= (balance_cancel actions' [] γ)); autorewrite with list in H; exact H]
+   |assumption]].
+
+inversion IHtrace; subst.
+inversion Htrace. subst.
+
+Lemma allow_pop_only_if_push_at_end : forall rpds actions q γ,
+                                        Balanced_actions actions (actions' ++ [push_action γ])
+
+Admitted.
+*)
+Definition Is_root_reachable_via rpds actions q : Prop :=
+  clos_refl_trans_action_with_actions (rpds_rel rpds) (@Allow_SA Γ) [] (rpds_root rpds) actions q.
+
+Definition Root_reachable_state (sys : RPDS) (q : Q) : Prop :=
+  exists actions, Is_root_reachable_via sys actions q.
+
+Lemma allow_preserves_balance : forall (actions : list (Stack_Action Γ)) a κ
+                                      (Hbal : Balance_to_kont actions κ)
+                                      (Hallow : Allow_SAs (actions ++ [a])),
+                                 exists κ', Balance_to_kont (actions ++ [a]) κ'.
+Proof.
+  intros; inversion Hallow as [| | |actions']; listac;
+  destruct Hbal as [actions_ [? Hκ]].
+  exists κ, actions_; split;[eapply (drt_append _ H)|]; auto.
+  exists (γ::κ), (actions_ ++ [push_action γ]); split; [apply balance_actions_at_end|constructor];auto.
+  destruct (push_end_remains _ _ H) as [moo boo]; subst.
+  inversion Hκ as [|? ? κ']; listac.
+  exists κ', moo; split; auto.
+  cut (Balanced_actions (actions' ++ [push_action γ; pop_action γ])
+                        (moo ++ [push_action γ; pop_action γ])).
+  intro pathpart.
+  cut (Balanced_actions (moo ++ [push_action γ; pop_action γ]) moo);
+    [intro pathpart'; apply (drt_append pathpart pathpart')
+    |eapply drt_step; [eapply drt_refl | pose (grumble := (balance_cancel moo [])); simpl in grumble; rewrite app_nil_r in grumble; auto]].
+  pose (L := @balance_actions_at_end _ _ _ H [pop_action γ]); do 2 rewrite app_assoc_reverse in L; auto.
+Grab Existential Variables.
+eapply drt_step; [apply drt_refl | pose (L := (balance_eps actions [])); rewrite app_nil_r in L; auto].
+Qed.
+
+Lemma list_split_tail : forall A (l : list A), l = [] \/ exists l' a, l = l' ++ [a].
+Proof.
+  induction l;
+  [left
+  |inversion IHl as [Hnil|[l' [a' htail]]]; subst; right;
+   [exists [], a|exists (a :: l'), a']]; auto.
+Qed.
+
+Lemma Allow_SAs_prefix : forall A (l' l : list (Stack_Action A)),
+                           Allow_SAs (l ++ l') -> Allow_SAs l.
+Proof.
+  induction l'; intros;
+  [rewrite app_nil_r in H; auto
+  |pose (L := IHl' (l ++ [a])); rewrite app_assoc_reverse in L; apply L in H;
+   inversion H; listac; auto].
+Qed.  
+Lemma Allow_SA_segmentation : forall A (l l' : list (Stack_Action A)) a a',
+                                Allow_SA (l ++ [a] ++ l') a' ->
+                                Allow_SA l a.
+Proof.
+  intros.
+  hnf in H.
+  cut (Allow_SAs ((l ++ [a]) ++ (l' ++ [a']))).
+  intro H'; apply Allow_SAs_prefix in H'; auto.
+  rewrite app_assoc in *; auto.
+Qed.
+
+Lemma paths_preserve_balance : forall rpds actions0 q actions κ
+                                      (Hbal : Balance_to_kont actions0 κ)
+                                      (Hallow : match actions with
+                                                    nil => True
+                                                  | a::_ => Allow_SA actions0 a
+                                                end)
+                                      (q' : Q)
+                                      (Hpath :
+                                         clos_refl_trans_action_with_actions rpds (@Allow_SA Γ)
+                                                                             actions0 q actions q'),
+                                 exists κ', Balance_to_kont (actions0 ++ actions) κ'.
+  intros; induction Hpath as [|? ? ? ? ? ? [κ_ [actionsb [Hbal' Hκ]]] ? Hallow_].
+  exists κ; rewrite app_nil_r; auto.
+  inverts Hpath.
+  exact I.
+  case_eq actions1.
+  intro; subst; simpl; rewrite app_nil_r in *; auto.
+  intros a' actions' Heq; subst; simpl.
+  pose (Allow_SA_segmentation actions0 actions' a' H1); auto.
+  inversion Hallow_ as [| |? γ|? γ]; listac.
+  - exists κ_, actionsb; split;
+  [cut (Balanced_actions (actions0 ++ actions ++ [eps_action _]) (actions0 ++ actions));
+    [intro path; apply (drt_append path Hbal')
+    |eapply drt_step; [apply drt_refl | pose (L := (balance_eps (actions0 ++ actions) [])); rewrite app_nil_r in L;  try rewrite app_assoc]]
+  |]; auto.
+  - exists (γ::κ_), (actionsb ++ [push_action γ]); split;
+    [rewrite app_assoc; apply balance_actions_at_end|constructor]; auto.
+  - listac.
+    rewrite app_assoc, <- H0, <- app_assoc; simpl.
+    rewrite <- H0 in Hbal',Hallow_.
+    pose (L := (ex_intro (Balance_to_kont_P (κ0 ++ [push_action γ]) κ_) actionsb (conj Hbal' Hκ))).
+    pose (L' := (allow_preserves_balance _ L Hallow_)).
+    rewrite <- app_assoc in L'; auto.
+Qed.
+  
+Remark reachable_balances_to_kont :
+  forall rpds actions q, Is_root_reachable_via rpds actions q -> exists κ, Balance_to_kont actions κ.
+Proof.
+  intros ? ? ? H; hnf in H.
+  induction H as [|? ? ? ? ? ? [κ IH] ? Hallow].
+  exists [],[]; split; constructor.  
+  apply (@allow_preserves_balance _ _ _ IH) in Hallow; auto.
+Qed.
+
+Definition frame_appears_in (γ : Γ) (actions : list (Stack_Action Γ)) : Prop :=
+  Exists (fun γa => match γa with
+                        eps_action => False
+                      | push_action γ' => γ = γ'
+                      | pop_action γ' => γ = γ'
+                    end) actions.
+
+Definition Root_reachable_frame (rpds : RPDS) (γ : Γ) : Prop :=
+  exists actions q, Is_root_reachable_via rpds actions q /\ frame_appears_in γ actions.
+
+Definition Balanced_path_with (rpds : RPDS) (q q' : Q) (actions0 actions : list (Stack_Action Γ)) :=
+  clos_refl_trans_action_with_actions (rpds_rel rpds) (@Allow_SA Γ) actions0 q actions q'
+  /\ Balanced_actions actions [].
+Hint Unfold Balanced_path_with.
+
+Definition Balanced_path (rpds : RPDS) (q q' : Q) :=
+  exists actions0, Is_root_reachable_via rpds actions0 q /\
+                   exists actions, Balanced_path_with rpds q q' actions0 actions.
+
+Definition NE_Balanced_path (rpds : RPDS) (q q' : Q) :=
+  exists actions0, Is_root_reachable_via rpds actions0 q /\
+                   exists actions, actions <> nil /\ Balanced_path_with rpds q q' actions0 actions.
+
+Inductive Epsilon_closure (rpds : RPDS) : relation Q -> Prop :=
+  eps_closure : forall δε,
+                  (forall s s',
+                     (δε s s' <-> Balanced_path rpds s s')) ->
+                  Epsilon_closure rpds δε.
+
+Remark good_root : forall rpds (isQ' : Q -> bool) (goodQ : forall q, (isQ' q) <-> Root_reachable_state rpds q),
+                     isQ' (rpds_root rpds).
+intros; destruct (goodQ (rpds_root rpds)) as [_ H]; apply H; exists []; apply rtaa_refl.
+Qed.
+
+Inductive RPDS_compaction : RPDS -> RPDS -> Type :=
+  compact_intro :
+    forall rpds (isQ' : Q -> bool) (isΓ' : Γ -> bool),
+      `{forall (GoodQ : (forall q, (isQ' q) <-> Root_reachable_state rpds q)),
+        (forall γ, (isΓ' γ) <-> Root_reachable_frame rpds γ) ->
+        (forall q γa q', (δ' q γa q') <-> exists actions, Is_root_reachable_via rpds actions q /\
+                                                          (rpds_rel rpds q γa q') /\
+                                                          exists κ, Balance_to_kont (actions ++ [γa]) κ) ->
+    RPDS_compaction rpds (rpds_intro (pds_intro isQ' isΓ' δ' prf1 prf2 prf3)
+                                     (rpds_root rpds)
+                                     (good_root isQ' GoodQ))}.  
+
+Lemma compaction_reachability_with_actions :
+  forall rpds crpds,
+    RPDS_compaction rpds crpds ->
+    forall actions q,
+      Is_root_reachable_via rpds actions q <-> Is_root_reachable_via crpds actions q.
+Proof.
+  intros rpds crpds Hcompact actions q;
+  inversion_clear Hcompact as [? isQ' isΓ' δ' prf1 prf2 prf3 Qreach Γreach edgereach]; subst;
+  split; intro Hreach.
+  - hnf in Hreach; rewrite rtaa_family_iff_index in Hreach;
+  induction Hreach as [|y z actions γa Hreach IH Hstep];[constructor|rewrite <- rtaa_family_iff_index in Hreach];
+  eapply rtaa_step; eauto;
+  rewrite edgereach;
+  exists actions; repeat split; auto;
+  inversion H as [| |? γ|actions' γ]; simpl in *; subst; listac;
+  try solve
+  [exists κ,actions_; split; listac;
+   [eapply drt_append;
+     [eapply balance_actions_at_end; eauto
+     |eapply drt_step; [constructor|rewrite <- app_nil_r; eapply (balance_eps actions_ [])]]
+   |auto]
+  |exists (γ::κ),(actions_++[push_action γ]); split;
+   [eapply balance_actions_at_end|constructor]; auto];
+    (* part way *)
+    destruct (reachable_balances_to_kont IH) as [? Hbal];
+    pose (L := (allow_preserves_balance _ Hbal H));
+    try rewrite app_assoc_reverse in L; auto.
+
+  - hnf in Hreach; rewrite rtaa_family_iff_index in Hreach;
+  induction Hreach as [|? ? ? ? Hreach IH Hstep];[constructor|rewrite <- rtaa_family_iff_index in Hreach];
+    rewrite edgereach in Hstep;destruct Hstep as [? [? [yredz mumble]]];
+    inverts H; listac; try solve
+      [eapply rtaa_step; [exact IH |  |]; auto].
+    pose (L := @rtaa_step _ _ (rpds_rel rpds) (@Allow_SA Γ) [] (rpds_root rpds) y z (κ ++ [push_action γ]) (pop_action γ) IH yredz H).
+    rewrite app_assoc_reverse in L; simpl in L; auto.
+Qed.
+
+Lemma compaction_reachability_with_actions' :
+  forall rpds crpds,
+    RPDS_compaction rpds crpds ->
+    forall actions q actions' q',
+      Is_root_reachable_via rpds actions q /\
+      clos_refl_trans_action_with_actions (rpds_rel rpds) (@Allow_SA Γ) actions q actions' q'
+      <-> Is_root_reachable_via crpds actions q /\
+          clos_refl_trans_action_with_actions (rpds_rel crpds) (@Allow_SA Γ) actions q actions' q'.
+Proof.
+  intros rpds crpds Hcompact actions q;
+  inversion Hcompact as [? isQ' isΓ' δ' prf1 prf2 prf3 Qreach Γreach edgereach]; subst;
+  split; intros [Hreach Hreach'].
+  - split;
+    [rewrite <- compaction_reachability_with_actions; [exact Hreach|exact Hcompact]
+    |]. 
+    rewrite rtaa_family_iff_index in Hreach';
+      induction Hreach' as [|y z actions_ γa Hreach' IH Hstep];
+      [constructor
+      |rewrite <- rtaa_family_iff_index in Hreach'].
+  destruct (reachable_balances_to_kont Hreach) as [κr Hr];
+  pose (use := @paths_preserve_balance (rpds_rel rpds) actions q actions_ _ Hr);
+  inversion H as [| |? γ|actions' γ]; simpl in *; subst; listac.
+  (* empty case *)
+  case_eq actions_; intros; subst;
+    [inversion Hreach'; listac; subst|].
+  rewrite app_nil_r in H.
+  eapply rtaa_step; [exact IH| |].
+  rewrite edgereach; exists actions; repeat split; auto.
+  specialize (use I _ Hreach'); rewrite app_nil_r in use.
+  destruct use as [κ' Hbal]; apply (allow_preserves_balance _ Hbal H).
+  rewrite app_nil_r; auto.
+
+  eapply rtaa_step;
+    [exact IH
+    |rewrite edgereach; exists (actions ++ (s :: l)); repeat split; 
+     try solve [auto|eapply (rtaa_append Hreach _ _ Hreach')]
+    |auto].
+  (* eps action balances to kont *)
+  destruct (reachable_balances_to_kont Hreach) as [κ0 Hbal];
+  destruct (s :: l);
+    [specialize (use I y Hreach');
+      rewrite app_nil_r in *;
+      destruct use as [κ' [actions' [Hbal_ Hform_]]];
+      exists κ', actions'; split;
+      [eapply (drt_append _ Hbal_)|auto]
+    |cut (Allow_SA actions s0);
+      [intro mum; destruct (use mum y Hreach') as [κ_ [actions_ [Hbal_ Hform_]]];
+       exists κ_,actions_; split; [eapply (drt_append _ Hbal_)|]; auto
+      |pose (use' := @Allow_SA_segmentation _ actions l0 s0 (eps_action _) H); auto]].
+  (* push case *)
+  eapply rtaa_step; [exact IH|rewrite edgereach; exists (actions ++ actions_); repeat split|]; auto.
+  
+  case_eq actions_; intros; subst;
+  [inversion Hreach'; listac; subst; rewrite app_nil_r
+  |listac; eapply (rtaa_append Hreach _ _ Hreach')]; auto.
+
+  case_eq actions_; intros; subst;
+  [rewrite app_nil_r in *; listac;
+   destruct Hr as [actionsb [Hbal Hform]];
+   exists (γ::κr),(actionsb++[push_action γ]); split; [apply balance_actions_at_end|constructor];auto
+  |cut (Allow_SA actions s);
+    [intro Ha; destruct (use Ha y Hreach') as [κ' [actionsb [Hbal Hform]]];
+     listac;
+     exists (γ::κ'),(actionsb ++ [push_action γ]); split; [apply balance_actions_at_end|constructor]; auto
+    |apply (Allow_SA_segmentation _ _ _ H)]].
+
+  (* pop case *)
+  eapply rtaa_step; [exact IH|rewrite edgereach; exists (actions ++ actions_); repeat split |]; auto.
+  case_eq actions_; intros; subst;
+  [inversion Hreach'; listac; subst; rewrite app_nil_r
+  |listac; eapply (rtaa_append Hreach _ _ Hreach')]; auto.
+
+  case_eq actions_; intros; subst;
+  [rewrite app_nil_r in *;
+    apply (allow_preserves_balance _ Hr H)
+  |].
+  simpl in use.
+  cut (Allow_SA actions s);[
+      intro Ha; destruct (use Ha _ Hreach') as [κ' [actionsb [Hbal Hform]]]
+     |].
+  cut (actions ++ s :: l = actions' ++ [push_action γ]);
+    [
+  intros rew; subst; rewrite rew,<- app_assoc in *; simpl;
+  destruct (push_end_remains _ _ Hbal) as [moo boo]; subst;
+  inversion Hform; listac;
+  exists κ, moo; split; auto;
+  cut (Balanced_actions (actions' ++ [push_action γ; pop_action γ]) (moo ++ [push_action γ; pop_action γ]));
+    [intro pathpart;
+      cut (Balanced_actions (moo ++ [push_action γ; pop_action γ]) moo);
+      [intro pathpart'; apply (drt_append pathpart pathpart')
+      |eapply drt_step; [apply drt_refl | pose (L:= (balance_cancel moo [] γ)); repeat rewrite app_nil_r in L]]
+    |pose (L := balance_actions_at_end Hbal [pop_action γ]); repeat rewrite app_assoc_reverse in L]; auto
+  |cut (actions' ++ [push_action γ; pop_action γ] = (actions' ++ [push_action γ]) ++ [pop_action γ]);
+    [intro Heq; listac
+    |rewrite app_assoc_reverse] ;auto].
+  apply (@Allow_SA_segmentation _ actions l s _ H).
+
+  - split; [rewrite <- compaction_reachability_with_actions in Hreach; [exact Hreach|exact Hcompact]|].
+    rewrite rtaa_family_iff_index in Hreach';
+    induction Hreach' as [|? ? ? ? Hreach_ IH Hstep];[constructor|rewrite <- rtaa_family_iff_index in Hreach_].
+    eapply rtaa_step; [exact IH |rewrite edgereach in Hstep; destruct Hstep as [? [? [? ?]]] | ]; auto.
+Grab Existential Variables.
+simpl; apply (Allow_SA_segmentation _ l s H).
+discriminate.
+simpl; apply (Allow_SA_segmentation _ l s H).
+discriminate.
+eapply drt_step; [apply drt_refl | pose (L := balance_eps (actions ++ s0 :: l0) []); repeat rewrite app_nil_r in L]; auto.
+eapply drt_step; [apply drt_refl | pose (L := balance_eps actions []); repeat rewrite app_nil_r in L]; auto.
+simpl; apply (Allow_SA_segmentation _ l s H).
+discriminate.
+Qed.
+
+Lemma eps_closure_in_compaction : forall rpds crpds δε, Epsilon_closure rpds δε ->
+                                                       RPDS_compaction rpds crpds ->
+                                                       Epsilon_closure crpds δε.
+Proof.
+  intros rpds crpds δε Heps Hcompact;
+  pose (HC := compaction_reachability_with_actions' Hcompact).
+  inversion_clear Heps as [? epsinv];
+  constructor.
+  intros s s'; split;[intro Hε|intros [Hreachs Hbalanced]].
+
+  rewrite epsinv in Hε; destruct Hε as [actions0 [reach0 [actions [path hbal]]]].
+
+  pose (both := conj reach0 path); rewrite HC in both.
+  destruct both; exists actions0; split; [|exists actions];auto.
+
+  rewrite epsinv.
+  destruct Hbalanced as [reachs [actions [path bal]]].
+  pose (both := conj reachs path); rewrite <- HC in both.
+  destruct both; exists Hreachs; split; [|exists actions]; auto.
+Qed.
+  
+Definition WorkEdge := (Q * Γ * Q)%type.
+Definition EpsEdge := (Q * Q)%type.
+
+Inductive Working_rpds : Type :=
+  working_rpds : forall (Qs : list Q)
+                        (pushE : list WorkEdge)
+                        (popE : list WorkEdge)
+                        (epsE : list EpsEdge)
+                        (q0 : Q)
+                        (H : list EpsEdge)
+                 (ΔQs : list Q)
+                 (ΔpushE : list WorkEdge)
+                 (ΔpopE : list WorkEdge)
+                 (ΔepsE : list EpsEdge)
+                 (ΔH : list EpsEdge),
+                   Working_rpds.
+
+Inductive Qs_contained (Qs : set Q) (ΔQs : set Q) (isQ : Q -> bool) : Prop :=
+  qs_contained_intro : (forall q, In q Qs \/ In q ΔQs -> isQ q) -> Qs_contained Qs ΔQs isQ.
+
+Inductive Edges_contained (Es : set WorkEdge) (ΔEs : set WorkEdge) (action : Γ -> Stack_Action Γ)
+          (δ : action_relation Q (Stack_Action Γ)) : Prop :=
+  es_contained_intro : (forall q γ q', In (q,γ,q') Es \/ In (q,γ,q') ΔEs -> δ q (action γ) q') -> 
+                       Edges_contained Es ΔEs action δ.
+
+Inductive Eps_contained (Es : set EpsEdge) (ΔEs : set EpsEdge) (δ : action_relation Q (Stack_Action Γ)) : Prop :=
+  eps_contained_intro : (forall q q', In (q,q') Es \/ In (q,q') ΔEs -> δ q (eps_action Γ) q') ->
+                        Eps_contained Es ΔEs δ.
+
+Inductive EpsC_contained (Es : set EpsEdge) (ΔEs : set EpsEdge) (δε : relation Q) : Prop :=
+  epsc_contained_intro : (forall q q', In (q,q') Es \/ In (q,q') ΔEs -> δε q q') -> EpsC_contained Es ΔEs δε.
+
+Inductive Working_contained : Working_rpds -> forall (rpds : RPDS) (δε : relation Q),
+                                                Epsilon_closure rpds δε -> Prop :=
+  contained_intro : forall Qs pushE popE epsE q0 H ΔQs ΔpushE ΔpopE ΔepsE ΔH
+                    (isQ : Q -> bool) (isΓ : Γ -> bool) (δ : action_relation Q (Stack_Action Γ)) prf1 prf2 prf3
+                    q0isQ
+                    (δε : relation Q) is_epsclosed,
+                      Qs_contained Qs ΔQs isQ ->
+                      Edges_contained pushE ΔpushE (@push_action Γ) δ ->
+                      Edges_contained popE ΔpopE (@pop_action Γ) δ ->
+                      Eps_contained epsE ΔepsE δ ->
+                      EpsC_contained H ΔH δε ->
+                      @Working_contained
+                        (working_rpds Qs pushE popE epsE q0 H ΔQs ΔpushE ΔpopE ΔepsE ΔH)
+                        (rpds_intro (pds_intro isQ isΓ δ prf1 prf2 prf3) q0 q0isQ)
+                        δε is_epsclosed.
+
+Section FiniteAssumptions.
+Variables (Qeq_dec : dec_type Q) (Γeq_dec : dec_type Γ) (rpds : RPDS).
+Definition pullback_true {A} (f : A -> bool) := sigT (fun a => f a = true).
+Variables (fin_Q : NeFiniteT (pullback_true (pds_Q (rpds_pds rpds))))
+          (fin_Γ : NeFiniteT (pullback_true (pds_Γ (rpds_pds rpds)))).
+Variables (δsp : Q -> list (Q * (Stack_Action Γ))) (* eval *)
+          (δp : Q -> Γ -> list Q) (* apply, though can't push immediately after pop *)
+          (δsp_correspondence :
+             forall q q',
+               (((rpds_rel rpds) q (eps_action Γ) q') <-> In (q', (eps_action Γ)) (δsp q)) /\
+               forall γ, (((rpds_rel rpds) q (push_action γ)  q') <-> In (q', (push_action γ)) (δsp q)) /\
+                         (In (q', (pop_action γ)) (δsp q) -> False))
+          (δp_correspondence : forall q γ q', ((rpds_rel rpds) q (pop_action γ) q') <-> In q' (δp q γ)).
+
+Definition Edge := (Q * (Stack_Action Γ) * Q)%type.
+Definition PushPred := (Q * Γ)%type.
+Hint Immediate Qeq_dec Γeq_dec.
+Definition stackact_eq_dec : dec_type (Stack_Action Γ). decide equality. Defined.
+Hint Immediate stackact_eq_dec.
+Definition edge_eq_dec : dec_type Edge. do 2 decide equality. Defined.
+Definition eps_edge_eq_dec : dec_type EpsEdge. decide equality. Defined.
+Definition work_edge_eq_dec : dec_type WorkEdge. do 2 decide equality. Defined.
+Definition QΓ_eq_dec : dec_type PushPred. decide equality. Defined.
+Hint Immediate edge_eq_dec eps_edge_eq_dec work_edge_eq_dec.
+Definition working_eq_dec : dec_type Working_rpds. repeat decide equality. Defined.
+
+Fixpoint push_eps_aux (q0 : Q) (todo : list (Q * (Stack_Action Γ)))
+         (actions : list WorkEdge) (epss : list EpsEdge) (states : list Q) :=
+  match todo with
+      nil => (actions, epss, states)
+    | (q,γa)::todo' => match γa with
+                           eps_action => push_eps_aux q0 todo' actions ((q0,q)::epss) (q::states)
+                         | push_action γ => push_eps_aux q0 todo' ((q0,γ,q)::actions) epss (q::states)
+                         (* impossible *)
+                         | pop_action _ => push_eps_aux q0 todo' actions epss states
+                       end
+  end.
+
+Lemma push_eps_contained_inv :
+  forall q0 todo actions epss states,
+    (forall q, In q states -> rpds_Q rpds q) ->
+    (forall γa q, In (q,γa) todo -> ((rpds_rel rpds) q0 γa q)) ->
+    (forall q γ q', In (q,γ,q') actions -> (rpds_rel rpds) q (push_action γ) q') ->
+    (forall q q', In (q,q') epss -> (rpds_rel rpds) q (eps_action _) q') ->
+    match push_eps_aux q0 todo actions epss states with
+        (actions',epss',states') =>
+        (forall q, In q states' -> rpds_Q rpds q) /\
+        (forall q γ q', In (q,γ,q') actions' -> (rpds_rel rpds) q (push_action γ) q') /\
+        (forall q q', In (q,q') epss' -> (rpds_rel rpds) q (eps_action _) q')
+    end.
+Proof.
+  destruct rpds as [[isQ isΓ δ prf1 prf2 prf3] s0 ?].
+
+  induction todo as [|(q,γa) todo_ IH]; intros actions epss states Hstates Htodo Hactions Hepss; repeat split; auto.
+  cut (forall γa q, In (q, γa) todo_ -> δ q0 γa q);[|intros; apply Htodo; right; auto].
+  intro HT; simpl; destruct γa as [|γ|γ];
+  [| |apply IH; solve [auto | intros γa q' Hin; apply Htodo; right; auto]].
+  (* eps case *)
+  case_eq (push_eps_aux q0 todo_ actions ((q0, q) :: epss) (q :: states)).
+  specialize (IH actions ((q0,q)::epss) (q::states)).
+  cut (forall q', In q' (q :: states) -> isQ q');
+    [|intros q'' [Heq''|Hrest];
+       [pose (Htodo' := Htodo (eps_action _) q (or_introl (eq_refl _)));
+         subst; apply prf1 in Htodo'; intuition auto
+       |apply Hstates; auto]].
+  intro HQ; specialize (IH HQ HT Hactions).
+  cut (forall q_ q', In (q_,q') ((q0,q)::epss) -> δ q_ (eps_action _) q');
+    [|intros q_ q_' [eq_|Hrest];
+       [injects eq_;apply (Htodo (eps_action _) q_' (or_introl (eq_refl _)))
+       |apply Hepss; auto]].
+  intro HE; specialize (IH HE).
+  intros [actions' epss'] states' Hreceq; rewrite Hreceq in IH;
+  destruct IH as [IHQ [IHE IHε]]; repeat split; auto.
+  (* push case *)
+  case_eq (push_eps_aux q0 todo_ ((q0,γ,q)::actions) epss (q :: states)).
+  specialize (IH ((q0,γ,q)::actions) epss (q :: states)).
+  cut (forall q', In q' (q :: states) -> isQ q');
+    [|intros q'' [Heq''|Hrest];
+       [pose (Htodo' := Htodo (push_action γ) q (or_introl (eq_refl _)));
+         subst; apply prf2 in Htodo'; intuition auto
+       |apply Hstates; auto]].
+  intro HP; specialize (IH HP HT).
+  cut (forall q' γ' q'', In (q', γ',q'') ((q0,γ,q)::actions) -> δ q' (push_action γ') q'');
+    [|intros ? ? ? [Heq|Hrest];[injects Heq;apply (Htodo (push_action γ') q'' (or_introl (eq_refl _)))
+                               |apply Hactions; auto]].
+  intro HA; specialize (IH HA Hepss).
+  intros [actions' epss'] states' Hreceq; rewrite Hreceq in IH; 
+  destruct IH as [IHQ [IHE IHε]]; repeat split; auto.
+Qed.
+
+Definition sprout (q : Q) : (list WorkEdge * list EpsEdge * list Q):=
+  push_eps_aux q (δsp q) nil nil nil.
+
+Lemma sprout_contained_inv :
+  forall q,
+    match sprout q with
+        (actions',epss',states') =>
+        (Forall (rpds_Q rpds) states') /\
+        (Forall (fun edge => match edge with (q, γ, q') => (rpds_rel rpds) q (push_action γ) q' end) actions') /\
+        (Forall (fun eedge : EpsEdge => let (q,q'):=eedge in rpds_rel rpds q (eps_action _) q') epss')
+    end.
+Proof.
+  intro q0; unfold sprout. 
+  (* Have to give nil's types due to rewriting bug *)
+  pose (L := @push_eps_contained_inv q0 (δsp q0) (@nil WorkEdge) (@nil EpsEdge) [] (fun q H => match H with end)).
+  cut (forall γa q, In (q,γa) (δsp q0) -> rpds_rel rpds q0 γa q).
+  intro Htodo; specialize (L Htodo (fun x y z H => match H with end) (fun x y H => match H with end)).  
+  case_eq (push_eps_aux q0 (δsp q0) [] [] []); intros [actions' eps'] states' Heq.
+  rewrite Heq in L; destruct L as [Hstates [Hactions Heps]].
+  repeat rewrite Forall_forall; repeat split; auto.
+  intros [[q γ] q']; apply Hactions.
+  intros [q q']; apply Heps.
+  intros γa q Hin;
+  destruct (δsp_correspondence q0 q) as [Heps Haction];
+   destruct γa as [|γ|γ];
+   [rewrite Heps
+   |destruct (Haction γ) as [Hpush Hpop]; rewrite Hpush
+   |destruct (Haction γ) as [Hpush Hpop]; elimtype False; apply Hpop]; auto.
+Qed.
+
+Definition eps_grab (q : Q) (H : list EpsEdge) (acc : set Q) (backwards : bool) : set Q :=
+  fold_left (fun acc (pair : Q * Q) =>
+               let (q',q'') := pair in
+               if backwards then
+                 (if (Qeq_dec q q'') then
+                    set_add Qeq_dec q' acc
+                  else acc)
+               else (if (Qeq_dec q q') then
+                       set_add Qeq_dec q'' acc
+                     else acc)) H acc.
+Definition eps_pred (q : Q) (H : list EpsEdge) : list Q :=
+  eps_grab q H nil true.
+
+Definition eps_succ (q : Q) (H : list EpsEdge) : list Q :=
+  eps_grab q H nil false.
+
+Lemma eps_grab_acc : forall q (backwards : bool) H acc q',
+                       In q' acc -> In q' (eps_grab q H acc backwards).
+Proof.
+  induction H as [|(q',q'') H' IH]; intros acc q_ Hin;
+  auto; simpl.
+  destruct backwards;
+    [destruct (Qeq_dec q q'')|destruct (Qeq_dec q q')]; subst;
+  apply IH; try solve [apply set_add_intro1; auto | auto].
+Qed.
+
+Lemma eps_grab_correct : forall q (backwards : bool) H acc,
+                           if backwards then
+                             forall q', In (q',q) H \/ In q' acc <-> In q' (eps_grab q H acc true)
+                           else
+                             forall q', In (q,q') H \/ In q' acc <-> In q' (eps_grab q H acc false).
+Proof.
+  induction H as [|(q',q'') H' IH]; intro acc; destruct backwards; try solve [intuition; listac].
+  intros q_; split; intro H.
+  - inversion H as [[topH|restH]|inAcc];
+    [simpl; injects topH; split_refl Qeq_dec q;
+     rewrite <- IH; right; apply set_add_intro2; auto;
+     pose (restH' := or_introl (In q_ acc) restH);
+     rewrite IH in restH'
+     |simpl;
+       destruct (Qeq_dec q q'');rewrite <- IH;
+       [subst;left;auto|left; auto]
+     |simpl;
+       destruct (Qeq_dec q q'');rewrite <- IH;subst;
+       right;[apply set_add_intro1|];auto].
+  - simpl in H; destruct (Qeq_dec q q''); subst.
+    rewrite <- IH in H; inversion H as [inH|inacc];
+    [left;right;auto|].
+    apply set_add_elim in inacc; inversion inacc as [Heq|Hin];
+    [subst;left;left|]; auto.
+    rewrite <- IH in H; inversion H;[subst;left;right|right]; auto.
+  - intros q_; split; intro H; simpl.
+    inversion H as [[topH|restH]|inacc];
+      [injects topH; split_refl Qeq_dec q;
+       rewrite <- IH; right; apply set_add_intro2; auto
+      |destruct (Qeq_dec q q'); subst; rewrite <- IH; left; auto
+      |destruct (Qeq_dec q q'); subst;
+       rewrite <- IH; right; [apply set_add_intro1|]; auto].
+    simpl in H.
+    destruct (Qeq_dec q q'); subst; 
+    rewrite <- IH in H;
+    inversion H as [inH|inacc];
+    [left; right
+    |destruct (set_add_elim _ _ _ _ inacc) as [Heq|Hacc];
+      [subst; left; left|right]; auto
+    | |]; auto.
+Qed.
+
+Lemma eps_pred_correct : forall q H q', In (q',q) H <-> In q' (eps_pred q H).
+Proof.
+  intros; pose (L := @eps_grab_correct q true H nil q');
+  simpl in L; split; intro X;
+  [rewrite <- L;left; auto
+  |rewrite <- L in X; inversion X; [auto|contradiction]].
+Qed.
+
+Lemma eps_succ_correct : forall q H q', In (q,q') H <-> In q' (eps_succ q H).
+Proof.
+  intros; pose (L := @eps_grab_correct q false H nil q');
+  simpl in L; split; intro X;
+  [rewrite <- L;left; auto
+  |rewrite <- L in X; inversion X; [auto|contradiction]].
+Qed.
+
+Definition add_pops_from_pushes (s : Q) (q' : Q) (γ : Γ)
+           (todo : list Q)
+           (acc : list WorkEdge * list EpsEdge * list Q) :=
+  fold_left (fun acc' q'' =>
+               match acc' with
+                   (ΔE,ΔH,ΔQ) =>
+                   (* always pop actions *)
+                   ((set_add work_edge_eq_dec (q', γ,q'') ΔE),
+                    (set_add eps_edge_eq_dec (s,q'') ΔH),
+                    (set_add Qeq_dec q'' ΔQ))
+               end)
+            todo acc.
+Check Balanced_path_with.
+
+Lemma push_balance_pop : forall actions (γ : Γ), Balanced_actions actions [] ->
+                                           Balanced_actions (push_action γ :: actions ++ [pop_action γ]) [].
+Proof.
+  intros; hnf.
+  cut (Balanced_actions ((push_action γ :: actions) ++ [pop_action γ]) ([push_action γ] ++ [pop_action γ]));
+    [|apply balance_actions_at_end;
+       hnf; pose (L := balance_actions_at_front H [push_action γ]); rewrite app_nil_r in L; auto].
+  intro path;simpl in path.
+  cut (Balanced_actions [push_action γ; pop_action γ] []).
+  intro path'.
+  apply (drt_append path path').
+  eapply drt_step; [apply drt_refl|apply (balance_cancel [] [])].
+Qed.
+
+Lemma push_balance_pop' : forall actions0 q actions q' γ qprev q'post, Balanced_path_with rpds q q' (actions0 ++ [push_action γ])
+                                                                            actions ->
+                                                         rpds_rel rpds qprev (push_action γ) q ->
+                                                         rpds_rel rpds q' (pop_action γ) q'post ->
+                                                         Balanced_path_with rpds qprev q'post actions0 (actions ++ [pop_action γ]).
+Admitted.
+
+Lemma add_pops_from_pushes_contained_inv :
+  forall s q'prev q' γ δε
+         (εclosure : Epsilon_closure rpds δε)
+         (push_edge : rpds_rel rpds s (push_action γ) q'prev)
+         (q'path : δε q'prev q')
+         (reachs : Root_reachable_state rpds s),
+    forall todo ΔE ΔH ΔQ,
+      (forall q, In q todo -> rpds_rel rpds q' (pop_action γ) q /\
+      Root_reachable_state rpds q) ->
+      (forall q γ q', In (q,γ,q') ΔE -> rpds_rel rpds q (pop_action γ) q') ->
+      (forall q q', In (q,q') ΔH -> NE_Balanced_path rpds q q') ->
+      (forall q, In q ΔQ -> rpds_Q rpds q) ->
+      match add_pops_from_pushes s q' γ todo (ΔE,ΔH,ΔQ) with
+          (ΔE,ΔH,ΔQ) => 
+          (forall q γ q', In (q,γ,q') ΔE -> rpds_rel rpds q (pop_action γ) q') /\
+          (forall q q', In (q,q') ΔH -> NE_Balanced_path rpds q q') /\
+          (forall q, In q ΔQ -> rpds_Q rpds q)
+      end.
+Proof.
+  induction todo as [|q todo' IH]; intros ΔE ΔH ΔQ.
+  intuition (simpl; auto).
+  intros HT HE HH HQ.
+  simpl.
+  case_eq (add_pops_from_pushes s q' γ todo' (set_add work_edge_eq_dec (q',γ,q) ΔE,
+                                              set_add eps_edge_eq_dec (s,q) ΔH,
+                                              set_add Qeq_dec q ΔQ)).
+  intros [ΔE' ΔH'] ΔQ' Heq.
+  specialize (IH (set_add work_edge_eq_dec (q',γ,q) ΔE) (set_add eps_edge_eq_dec (s,q) ΔH)
+                 (set_add Qeq_dec q ΔQ)).
+  cut (forall q, In q todo' -> rpds_rel rpds q' (pop_action γ) q /\ Root_reachable_state rpds q);
+    [intro HT'; specialize (IH HT')|intros q_ Hin; apply HT; right; auto].
+  cut (forall q_ γ_ q_', In (q_,γ_,q_') (set_add work_edge_eq_dec (q', γ, q) ΔE) ->
+                         rpds_rel rpds q_ (pop_action γ_) q_');
+    [intro HE'; specialize (IH HE')
+    |intros ? ? ? Hin; destruct (set_add_elim _ _ _ _ Hin) as [Heq_|HErest];
+      [injects Heq_; apply HT; left; reflexivity
+      |apply HE; auto]].
+  cut (forall q_ q_', In (q_,q_') (set_add eps_edge_eq_dec (s,q) ΔH) -> NE_Balanced_path rpds q_ q_');
+    [intro HH'; specialize (IH HH')
+    |intros ? ? Hin; destruct (set_add_elim _ _ _ _ Hin) as [Heq_|HHrest];[|apply HH; auto];
+     injects Heq_;
+     destruct (HT q (or_introl (eq_refl _))) as [Hstep [actions Hreach]];
+     inversion εclosure as [? Hbal]; subst].
+  Focus 2.
+  rewrite Hbal in q'path.
+  destruct q'path as [q'actions [q'reach [Hq'actions [Hq'path q'bal]]]].
+  destruct reachs as [reachsactions srootreach].
+  exists reachsactions; split; auto; exists (push_action γ :: Hq'actions ++ [pop_action γ]); split.
+  discriminate.
+  hnf.
+  apply push_balance_pop.
+  rewrite Hbal;
+     destruct reachs as [actionss Hreachs];
+     exists actionss; split; [assumption
+                             |]].
+  Focus 2.
+  rewrite Hbal in q'path; destruct q'path as [qactions [Hprevreach [prevactions [Hqreach Hprevbal]]]].
+  exists (push_action γ :: prevactions ++ [pop_action γ]);
+    split.
+  eapply (@rtaa_step _ _ _ _ _ s q' q (push_action γ :: prevactions) (pop_action γ)).
+  eapply (@rtaa_step _ _ _ _ _ s s q' [] (push_action γ));
+    [apply rtaa_refl
+    |
+    |rewrite app_nil_r; constructor;destruct Hreachs;[constructor|auto]].
+     |auto
+     |hnf;rewrite <- app_assoc; constructor;constructor; destruct Hreachs;[constructor|auto]]].
+  cut (forall q_, In q_ (set_add Qeq_dec q ΔQ) -> rpds_Q rpds q_);
+    [intro HQ'; specialize (IH HQ');
+     (* invisible, but still matters *)  
+     unfold WorkEdge,EpsEdge,set in Heq,IH; rewrite Heq in IH
+    |intros ? Hin; destruct (set_add_elim _ _ _ _ Hin) as [Heq_|HQrest];
+     [subst;
+       destruct rpds as [[isQ isΓ δ prf1 prf2 prf3] s0 ?];
+       destruct (HT q (or_introl (eq_refl _))) as [HTq _];
+       apply prf3 in HTq; intuition auto
+     |apply HQ;auto]].
+  destruct IH as [IHE [IHH IHQ]].
+  repeat split; auto.
+Qed.
+
+Definition add_pops_from (s : Q) (γ : Γ) (todo : list Q) (acc : list WorkEdge * list EpsEdge * list Q) :=
+  fold_left (fun acc' q' =>
+               add_pops_from_pushes s q' γ (δp q' γ) acc')
+            todo acc.
+
+Lemma add_pops_from_contained_inv :
+  forall s q' γ δε
+         (εclosure : Epsilon_closure rpds δε)
+         (push_edge : rpds_rel rpds s (push_action γ) q')
+         (reachs : Root_reachable_state rpds s),
+    forall todo ΔE ΔH ΔQ,
+      (forall q, In q todo -> rpds_rel rpds q' (pop_action γ) q /\
+                              Root_reachable_state rpds q) ->
+      (forall q γ q', In (q,γ,q') ΔE -> rpds_rel rpds q (pop_action γ) q') ->
+      (forall q q', In (q,q') ΔH -> δε q q') ->
+      (forall q, In q ΔQ -> rpds_Q rpds q) ->
+      match add_pops_from s γ todo (ΔE,ΔH,ΔQ) with
+          (ΔE,ΔH,ΔQ) => 
+          (forall q γ q', In (q,γ,q') ΔE -> rpds_rel rpds q (pop_action γ) q') /\
+          (forall q q', In (q,q') ΔH -> δε q q') /\
+          (forall q, In q ΔQ -> rpds_Q rpds q)
+      end.
+
+
+Definition add_push (H : list EpsEdge) (sγq : WorkEdge) :=
+  match sγq with
+      (s, γ, q) => add_pops_from s γ (eps_succ q H) (nil,nil,nil)
+  end.
+
+Definition pushes_to_acc (s' : Q) (E : list WorkEdge) (acc : list (Q * Γ)) :=
+  fold_left (fun acc edge =>
+               match edge with
+                   (q, γ, q') =>
+                   if (Qeq_dec s' q') then
+                     set_add QΓ_eq_dec (q,γ) acc
+                   else acc end) E acc.
+Definition pushes_to (s' : Q) (E : list WorkEdge) : list (Q * Γ) :=
+  pushes_to_acc s' E nil.
+
+Definition push_pred_acc (pushE : list WorkEdge) (s' : Q) (γ : Γ) (acc : list Q) :=
+  fold_left (fun acc edge =>
+               match edge with
+                   (q, γ', q') =>
+                   if (Γeq_dec γ γ') then
+                     if (Qeq_dec s' q') then
+                       set_add Qeq_dec q acc
+                     else acc
+                   else acc end) pushE acc.
+Definition push_pred (pushE : list WorkEdge) (s' : Q) (γ : Γ) :=
+  push_pred_acc pushE s' γ nil.
+
+Definition add_eps_from (q : Q) (base : list Q) (acc : list EpsEdge) :=
+  fold_left (fun acc' s => set_add eps_edge_eq_dec (s,q) acc') base acc.
+
+Definition add_pop_acc (q : Q) (γ : Γ) (pushE : list WorkEdge) (base : list Q) (acc : list EpsEdge) :=
+  fold_left (fun acc' s' => add_eps_from q (push_pred pushE s' γ) acc')
+            base acc.
+            
+Definition add_pop (H : list EpsEdge) (pushE : list WorkEdge) (s''γq : WorkEdge) :=
+  match s''γq with
+      (s'',γ,q) => add_pop_acc q γ pushE (eps_pred s'' H) nil
+  end.
+
+Definition add_empty (H : list EpsEdge) (pushE : list WorkEdge) (s''s''' : EpsEdge) :=
+  match s''s''' with
+      (s'',s''') =>
+      let post := (eps_succ s''' H) in
+      fold_left
+        (fun acc s' =>
+           fold_left
+             (fun (acc : list WorkEdge * list EpsEdge * list Q) s'''' =>
+                match acc with
+                    (ΔE,ΔH,ΔQ) =>
+                    fold_left
+                      (fun acc (sγ : PushPred) =>
+                         let (s,γ) := sγ in
+                         fold_left
+                           (fun (acc : list WorkEdge * list EpsEdge * list Q) q =>
+                              match acc with
+                                  (ΔE,ΔH,ΔQ) =>
+                                  (* all pop actions *)
+                                  (set_add work_edge_eq_dec (s'''', γ, q) ΔE,
+                                   set_add eps_edge_eq_dec (s,q) ΔH,
+                                   set_add Qeq_dec q ΔQ)
+                              end)
+                           (δp s'''' γ)
+                           acc)
+                      (pushes_to s' pushE)
+                      (ΔE, set_add eps_edge_eq_dec
+                                   (s',s''')
+                                   (set_add eps_edge_eq_dec
+                                            (s'',s'''')
+                                            (set_add eps_edge_eq_dec
+                                                     (s',s'''') ΔH)), ΔQ)
+                end)
+             post acc)
+        (eps_pred s'' H) (nil,nil,nil)
+  end.
+Definition WEQ_map {A} (f : A -> list WorkEdge * list EpsEdge * list Q) (l : list A) :=
+  triple_union_map work_edge_eq_dec eps_edge_eq_dec Qeq_dec f l.
+Definition wunion := set_union work_edge_eq_dec.
+Definition eunion := set_union eps_edge_eq_dec.
+Definition qunion := set_union Qeq_dec.
+Definition step_wrpds (wrpds : Working_rpds) :=
+  match wrpds with
+      working_rpds Qs pushE popE epsE q0 H ΔQs ΔpushE ΔpopE ΔepsE ΔH =>
+       match WEQ_map sprout ΔQs with
+           (ΔpushE0, ΔepsE0, ΔQ0) =>
+           match WEQ_map (add_push H) ΔpushE with
+               (ΔpopE1, ΔepsE1, ΔQ1) =>
+               let ΔepsE2 := union_map eps_edge_eq_dec (add_pop H pushE) ΔpopE in
+               match WEQ_map (add_empty H pushE) ΔH with
+                   (ΔpopE3, ΔepsE3,ΔQ3) =>
+                   let Qs' := qunion Qs ΔQs in
+                   let pushE' := wunion pushE ΔpushE in
+                   let popE' := wunion popE ΔpopE in
+                   let epsE' := eunion epsE ΔepsE in
+                   let H' := eunion H ΔH in
+                   let ΔpushE' := (set_diff work_edge_eq_dec ΔpushE0 pushE') in
+                   let ΔpopE' := (set_diff work_edge_eq_dec (wunion ΔpopE1 ΔpopE3) popE') in
+                   let ΔepsE' := (set_diff eps_edge_eq_dec ΔepsE0 epsE') in
+                   let ΔQs' := (set_diff Qeq_dec
+                                        (qunion ΔQ0 (qunion ΔQ1 (set_add Qeq_dec q0 ΔQ3)))
+                                        Qs') in
+                   let ΔH' := (set_diff eps_edge_eq_dec
+                                        (set_union eps_edge_eq_dec
+                                                   ΔepsE0
+                                                   (set_union eps_edge_eq_dec
+                                                              ΔepsE1
+                                                              (set_union eps_edge_eq_dec
+                                                                         ΔepsE2
+                                                                         ΔepsE3)))
+                                        H') in
+                   working_rpds Qs' pushE' popE' epsE' q0 H' ΔQs' ΔpushE' ΔpopE' ΔepsE' ΔH'
+               end
+           end
+       end
+  end.
+
+Definition Nonoverlapping {A} (s s' : list A) := forall a, In a s -> In a s' -> False.
+
+Inductive Working_Inv : Working_rpds -> forall rpds crpds δε,
+                                          Epsilon_closure rpds δε ->
+                                          RPDS_compaction rpds crpds -> Prop :=
+  inv_intro : forall Qs pushE popE epsE q0 H ΔQs ΔpushE ΔpopE ΔepsE ΔH
+                     rpds crpds δε is_epsclosed (is_compact : RPDS_compaction rpds crpds),
+                Nonoverlapping Qs ΔQs ->
+                Nonoverlapping pushE ΔpushE ->
+                Nonoverlapping popE ΔpopE ->
+                Nonoverlapping epsE ΔepsE ->
+                Nonoverlapping H ΔH ->
+                @Working_contained (working_rpds Qs pushE popE epsE q0 H ΔQs ΔpushE ΔpopE ΔepsE ΔH)
+                                   crpds δε (eps_closure_in_compaction is_epsclosed is_compact) ->
+                @Working_Inv (working_rpds Qs pushE popE epsE q0 H ΔQs ΔpushE ΔpopE ΔepsE ΔH)
+                             rpds crpds δε is_epsclosed is_compact.
+
+Lemma nonoverlapping_diff : forall A (eq_dec : dec_type A) (l' l : set A), Nonoverlapping l (set_diff eq_dec l' l).
+Proof.
+  induction l'.
+  intros ? ? ? bad; inversion bad.
+  intros l a' Hin Hindiff;
+  simpl in Hindiff.
+  case_eq (set_mem eq_dec a l); intros H; rewrite H in Hindiff;
+    [apply set_mem_correct1 in H;
+     apply (IHl' _ _ Hin Hindiff)
+    |apply set_mem_complete1 in H].
+  apply set_add_elim in Hindiff.
+  inversion Hindiff as [|H0];
+    [subst; contradiction
+    |apply (IHl' _ _ Hin H0)].
+Qed.
+
+Fixpoint ormap {A} (f : A -> bool) (l : list A) :=
+  match l with
+      nil => false
+    | a::l' => orb (f a) (ormap f l')
+  end.
+Lemma ormap_Exists : forall A (f : A -> bool) (l : list A), ormap f l <-> Exists (fun a => f a = true) l.
+Proof.
+  induction l; split; intro H; try solve [inversion H].
+  unfold ormap,orb in H;
+  case_eq (f a); intros Heq; rewrite Heq in H;
+    [apply Exists_cons_hd|rewrite IHl in H; apply Exists_cons_tl]; auto.
+  inversion H as [? ? Heq|? ? Heq].
+  unfold ormap,orb; rewrite Heq; reflexivity.
+  rewrite <- IHl in Heq; unfold ormap,orb.
+  rewrite Heq; destruct (f a); reflexivity.
+Qed.
+
+Lemma invariant : forall wrpds crpds δε
+                         (εclosure : Epsilon_closure rpds δε)
+                         (Hcompact : RPDS_compaction rpds crpds),
+                    Working_Inv wrpds εclosure Hcompact ->
+                    Working_Inv (step_wrpds wrpds) εclosure Hcompact.
+Proof.
+  destruct rpds as [[isQ isΓ δ prf1 prf2 prf3] s0 ?].
+  intros wrpds crpds δε εclosure Hcompact Hinv.
+  destruct crpds as [[isQc isΓc δc prf1c prf2c prf3c] cs0].
+  cut (cs0 = s0); [intro;subst|inverts Hcompact; reflexivity].
+  inversion Hcompact as [? ? ? ? δceps_good δcpush_good δcpop_good Qc_reach Γc_reach δc_reach]; subst.
+  inversion Hinv as [? ? ? ? ? ? ? ? ? ? ? ? ? ? ? ? Qnon pushnon popnon εnon hnon Hcontained]; subst;
+  inversion Hcontained as [? ? ? ? ? ? ? ? ? ? ? ? ? ? ? ? ? ? ? ? InQs InPush InPop InEps InH]; subst;
+  simpl.
+  
+  case_eq (WEQ_map sprout ΔQs); intros; subst;
+  case_eq p; intros; subst;
+  case_eq (WEQ_map (add_push H) ΔpushE); intros; subst;
+  case_eq p; intros; subst;
+  case_eq (WEQ_map (add_empty H pushE) ΔH); intros; subst;
+  case_eq p; intros; subst; apply inv_intro;
+  try solve [apply nonoverlapping_diff].
+  pose (Goal := @contained_intro
+                  (qunion Qs ΔQs) (wunion pushE ΔpushE) 
+        (wunion popE ΔpopE) (eunion epsE ΔepsE) s0 
+        (eunion H ΔH)
+        (set_diff Qeq_dec (qunion s (qunion s3 (set_add Qeq_dec s0 s6)))
+           (qunion Qs ΔQs))
+        (set_diff work_edge_eq_dec s1 (wunion pushE ΔpushE))
+        (set_diff work_edge_eq_dec (wunion s4 s7) (wunion popE ΔpopE))
+        (set_diff eps_edge_eq_dec s2 (eunion epsE ΔepsE))
+        (set_diff eps_edge_eq_dec
+           (set_union eps_edge_eq_dec s2
+              (set_union eps_edge_eq_dec s5
+                 (set_union eps_edge_eq_dec
+                    (union_map eps_edge_eq_dec (add_pop H pushE) ΔpopE) s8)))
+           (eunion H ΔH)) isQ isΓ δ prf1 prf2 prf3 _ δε is_epsclosed).
+  assert (isqc_imp_isq : forall q, isQc q -> isQ q)
+         by (intro q; rewrite Qc_reach0;
+             intros [? path];
+             inversion path as [|? ? ? ? ? ? Hstep]; subst; [auto|compute in Hstep; destruct a; [eapply prf1|eapply prf2|eapply prf3]]; eauto).
+  assert (subgoal1 :
+            forall q : Q,
+              In q (qunion Qs ΔQs) \/
+              In q
+                 (set_diff Qeq_dec (qunion s (qunion s3 (set_add Qeq_dec s0 s6)))
+                           (qunion Qs ΔQs)) -> isQ q).
+  - intros q [HqinU|Hqindiff];
+    [unfold qunion in HqinU; destruct (set_union_elim _ _ _ _ HqinU) as [HinQs|HinΔQs];
+     apply isqc_imp_isq; apply InQs; [left|right]; auto
+    |].
+  pose (Inqunion := set_diff_elim1 _ _ _ _ Hqindiff);
+  pose (NotInqunion := set_diff_elim2 _ _ _ _ Hqindiff);
+  unfold qunion in Inqunion; apply set_union_elim in Inqunion;
+  inversion_clear Inqunion as [Hqins|Hmid];
+    [|
+     unfold qunion in Hmid; apply set_union_elim in Hmid;
+     inversion_clear Hmid as [Hqins3|Hpost];
+     [|apply set_add_elim in Hpost;
+        inversion_clear Hpost as [qeqs0|Hqins6];
+        [subst; auto|]]].
+
+Admitted.
+
+Definition Qsize : nat :=
+  match fin_Q with
+      existT n _ => n
+end.
+Definition Γsize : nat :=
+  match fin_Γ with
+      existT n _ => n
+end.
+          
+Definition state_upperbound : nat := nat_expt 2 Qsize.
+Definition eps_upperbound : nat := nat_expt 2 (Qsize * Qsize).
+Definition edge_upperbound : nat := nat_expt 2 (Qsize * Qsize * Γsize).
+Definition working_measure (wrpds : Working_rpds) : {_ : nat & {_ : nat & nat}} :=
+  match wrpds with
+      working_rpds Qs pushE popE epsE q0 H ΔQs ΔpushE ΔpopE ΔepsE ΔH =>
+      existT _ 
+             (state_upperbound - (length ΔQs))
+             (existT _
+                     ((edge_upperbound - (length pushE)) +
+                      (edge_upperbound - (length popE)) +
+                      (eps_upperbound - (length epsE)))
+                     (eps_upperbound - (length H)))
+  end.
+Lemma nat_expt_pos : forall n m, n > 0 -> nat_expt n m > 0.
+induction m; intro;
+simpl. omega.
+specialize (IHm H); unfold gt in *; apply NPeano.Nat.mul_pos_pos; auto.
+Qed.
+Lemma termination_measure : forall wrpds,
+
+                              (step_wrpds wrpds = wrpds) \/
+                              lexprod _ (fun _ => _) lt (fun _ => lexprod _ (fun _ => _) lt (fun _ => lt))
+                                      (working_measure (step_wrpds wrpds))
+                                      (working_measure wrpds).
+Proof.
+  intro; destruct (working_eq_dec (step_wrpds wrpds) wrpds); [left; auto|right].
+  destruct wrpds; simpl;
+  case_eq (WEQ_map sprout ΔQs); intros; subst;
+  case_eq p; intros; subst;
+  case_eq (WEQ_map (add_push H) ΔpushE); intros; subst;
+  case_eq p; intros; subst;
+  case_eq (WEQ_map (add_empty H pushE) ΔH); intros; subst;
+  case_eq p; intros; subst; simpl.
+  destruct ΔQs.
+  destruct ΔpushE.
+  destruct ΔpopE.
+  destruct ΔepsE.
+  destruct ΔH.
+  simpl in n; case_eq (set_mem Qeq_dec q0 Qs); try solve [intro blah; rewrite blah in n; elimtype False; apply n; reflexivity].
+  intro notin; rewrite notin in n.
+  simpl in *; unfold WEQ_map,triple_union_map in H0,H1,H2; injects H0; injects H1; injects H2.
+  constructor; simpl; rewrite notin; simpl. 
+  unfold state_upperbound; pose (@nat_expt_pos 2 Qsize); cut (2 > 0); [intro|]; omega.
+  simpl in *; unfold WEQ_map,triple_union_map in H0,H1,H2; injects H0; injects H1.
+simpl in H2.
+apply right_lex.
+constructor.
+
+Theorem lfp_working_complete : 
+  
+End FiniteAssumptions.
+
+
+
+Remark example : Balanced_actions [eps_action bool ; push_action true ; eps_action bool ; pop_action true ; push_action false] [false].
+assert (subgoal:  Balanced_actions
+     [eps_action bool; push_action true; eps_action bool;
+      pop_action true] [])
+       by (apply (balance_eps [eps_action bool; push_action true] [pop_action true]),
+                 (balance_pushpop [eps_action bool] [] true);
+           autorewrite with list;
+           apply (balance_eps [] []);
+           simpl; constructor).
+apply (balance_push _ subgoal).
+Qed.
