reduction.v
@@ -1,0 +1,216 @@
+Require Import List Relation_Definitions Relation_Operators basic.
+Import ListNotations.
+Set Implicit Arguments.
+Definition action_relation (S A : Type) := S -> A -> S -> Prop.
+
+Section TraceClosures.
+
+Inductive clos_refl_trans_action (S A : Type) (R : action_relation S A) : S -> S -> Prop :=
+  rta_step : forall (x y z : S) (a : A),
+               clos_refl_trans_action R x y ->
+               R y a z -> clos_refl_trans_action R x z
+| rta_refl : forall x, clos_refl_trans_action R x x.
+
+Inductive direct_clos_refl_trans {A} (R : relation A) : A -> A -> Prop :=
+  drt_refl : forall x, direct_clos_refl_trans R x x
+| drt_step : forall x y z, direct_clos_refl_trans R x y ->
+                         R y z ->
+                         direct_clos_refl_trans R x z.
+
+
+Inductive Idirect_clos_refl_trans {A} (R : relation A) (x : A) : A -> Prop :=
+  idrt_refl : Idirect_clos_refl_trans R x x
+| idrt_step : forall y z, Idirect_clos_refl_trans R x y ->
+                         R y z ->
+                         Idirect_clos_refl_trans R x z.
+
+Ltac index_family istep step :=
+  let H := fresh in
+  intros; split; intro H; induction H; solve [constructor | eapply istep; eauto | eapply step; eauto].
+
+Lemma drt_family_iff_index : forall A (R : relation A) x y,
+                               direct_clos_refl_trans R x y <->
+                               Idirect_clos_refl_trans R x y.
+Proof.
+  index_family @idrt_step @drt_step.
+Qed.
+
+Lemma drt_prepend : forall A (R : relation A) x y,
+                      direct_clos_refl_trans R x y ->
+                      forall w, R w x ->
+                                       direct_clos_refl_trans R w y.
+Proof.
+  intros ? ? ? ? H; induction H; intros.
+  eapply drt_step; [constructor|auto].
+  eapply drt_step; [apply IHdirect_clos_refl_trans|]; auto.
+Qed.
+Lemma drt_append : forall A (R : relation A) x y,
+                     direct_clos_refl_trans R x y ->
+                     forall z,
+                     direct_clos_refl_trans R y z ->
+                     direct_clos_refl_trans R x z.
+Proof.
+  intros A R x y Hy; induction Hy; intros z' Hz.
+  assumption.
+  apply IHHy.
+  apply drt_prepend with (x := z); auto.
+Qed.
+
+Lemma drt_non_direct : forall A (R : relation A) x y,
+                         clos_refl_trans _ R x y <->
+                         direct_clos_refl_trans R x y.
+
+Proof.
+  intros; split; intro H; induction H.
+  eapply (drt_step y); [apply drt_refl|]; auto.
+  apply drt_refl.
+  apply (drt_append IHclos_refl_trans1 IHclos_refl_trans2).
+
+  apply rt_refl.
+  eapply (@rt_trans _ _ _ y z);[|apply rt_step]; auto.
+Qed.
+
+Section ActionTraces.
+Variables (Q Γ : Type) (R : action_relation Q Γ) (Allow : list Γ -> Γ -> Prop).
+
+Inductive clos_refl_trans_action_with_actions (actions0 : list Γ) : Q -> list Γ -> Q -> Prop :=
+  rtaa_refl : forall x, clos_refl_trans_action_with_actions actions0 x [] x
+| rtaa_step : forall (x y z : Q) actions (a : Γ),
+                clos_refl_trans_action_with_actions actions0 x actions y ->
+                R y a z ->
+                Allow (actions0 ++ actions) a ->
+                clos_refl_trans_action_with_actions actions0 x (actions ++ [a]) z.
+
+(* use indexed families for different induction schemes *)
+Inductive Iclos_refl_trans_action_with_actions (actions0 : list Γ) (x : Q) : list Γ -> Q -> Prop :=
+  irtaa_refl : Iclos_refl_trans_action_with_actions actions0 x [] x
+| irtaa_step : forall (y z : Q) actions (a : Γ),
+                Iclos_refl_trans_action_with_actions actions0 x actions y ->
+                R y a z ->
+                Allow (actions0 ++ actions) a -> Iclos_refl_trans_action_with_actions actions0 x (actions ++ [a]) z.
+
+Lemma rtaa_family_iff_index : forall actions0 x actions y,
+                                clos_refl_trans_action_with_actions actions0 x actions y <->
+                                Iclos_refl_trans_action_with_actions actions0 x actions y.
+Proof.
+  index_family irtaa_step rtaa_step.
+Qed.
+
+Lemma rtaa_head : forall actions0 x actions z, actions <> nil ->
+                                      clos_refl_trans_action_with_actions actions0 x actions z ->
+                                      match actions with
+                                          nil => False
+                                        | hd::tl => exists y, R x hd y /\ Allow actions0 hd /\ clos_refl_trans_action_with_actions (actions0 ++ [hd]) y tl z
+                                      end.
+Proof.
+  intros ? ? ? ? ? Hpath; induction Hpath; [bad_eq|].
+case_eq actions.
+- intro Hnil; subst;
+ inverts Hpath;[simpl; exists z; split; [assumption|constructor; [autorewrite with list in *; auto|constructor]]|destruct actions; discriminate].
+- intros a' actions' Haceq; subst;
+simpl.
+destruct IHHpath as [y' [xRy' [Hallow' pathy']]]; [discriminate|].
+exists y'; repeat split; try solve [assumption].
+eapply rtaa_step; [eauto|assumption|rewrite app_assoc_reverse; auto].
+Qed.
+
+Lemma rtaa_prepend : forall actions0 x actions y,
+                        forall a,
+                          clos_refl_trans_action_with_actions (actions0 ++ [a]) x actions y ->
+                          forall w, R w a x -> Allow actions0 a ->
+                                    clos_refl_trans_action_with_actions actions0 w (a::actions) y.
+Proof.
+  intros ? ? ? Aprop a Hy; induction Hy as [|x y z actions' a' noo IH Hred Hallow']; intros w Hw Hallow.
+  apply (@rtaa_step _ w w x [] a (rtaa_refl _ _) Hw); rewrite app_nil_r; assumption.
+  pose (L := (@rtaa_step _ w y z (a::actions') a' (IH _ Hw Hallow) Hred)).
+  apply L.
+  rewrite app_assoc_reverse in Hallow'.
+  auto.
+Qed.
+
+Definition Reassociate_allow {l l' l'' a} (P : Allow (l ++ l' ++ l'') a) : Allow ((l ++ l') ++ l'') a.
+rewrite app_assoc_reverse; exact P.
+Defined.
+
+Lemma rtaa_append : forall actions0 x actions y,
+                      clos_refl_trans_action_with_actions actions0 x actions y ->
+                     forall (actions' : list Γ) z,
+                       actions' <> nil ->
+                       match actions' with
+                           nil => False
+                         | hd::_ => Allow (actions0 ++ actions) hd
+                       end ->
+                       clos_refl_trans_action_with_actions (actions0 ++ actions) y actions' z ->
+                       clos_refl_trans_action_with_actions actions0 x (actions ++ actions') z.
+Proof.
+  intros ? ? ? ? Hy; induction Hy; intros actions' z' Hannil Hallow Hz.
+  rewrite app_nil_r in Hz; assumption.
+  rewrite app_assoc_reverse.
+  apply IHHy.
+  discriminate.
+  auto.
+  simpl.
+  apply rtaa_prepend with (x := z); auto.
+  rewrite app_assoc_reverse; auto.
+Qed.
+
+Inductive Sub_action_trace : 
+  forall actions0 q actions q',
+    clos_refl_trans_action_with_actions actions0 q actions q' ->
+    forall actions1 s actions' s',
+    clos_refl_trans_action_with_actions actions1 s actions' s' -> Prop :=
+empty_subtrace : forall actions0 actions s s'
+                        (H: clos_refl_trans_action_with_actions actions0
+                                                                s
+                                                                actions
+                                                                s'),
+                   Sub_action_trace
+                     (rtaa_refl (actions0 ++ actions) s') H
+|  step_subtrace :
+     forall actions0π sπ actionsπ s'π
+            (π : clos_refl_trans_action_with_actions actions0π sπ actionsπ s'π)
+            actions0 s actions s' a s''
+            (Hss' : clos_refl_trans_action_with_actions actions0 s actions s')
+            (Hsub : Sub_action_trace π Hss')
+            (Hstep : R s' a s'')
+            (Hallow : Allow (actions0 ++ actions) a),
+       Sub_action_trace π (rtaa_step Hss' Hstep Hallow)
+| ext_subtrace :
+    forall actions0' s actions s' actions0 s'' s'''
+           (sπ : clos_refl_trans_action_with_actions (actions0 ++ actions0') s actions s')
+           (π : clos_refl_trans_action_with_actions
+                   actions0 s''' (actions0' ++ actions) s')
+           a
+           (Hstep : R s' a s'')
+           (Hallow : Allow (actions0 ++ actions0' ++ actions) a),
+      Sub_action_trace sπ π ->
+      Sub_action_trace (rtaa_step sπ Hstep (Reassociate_allow Hallow)) (rtaa_step π Hstep Hallow).
+
+Generalizable All Variables.
+ Lemma subtrace_structure : `{forall (H : clos_refl_trans_action_with_actions
+                                           actions0 s actions s')
+                                    (H' : clos_refl_trans_action_with_actions actions0' s'' actions' s'''),
+                               Sub_action_trace H H' ->
+                               exists actionsL actionsR,
+                                 actions' = actionsL ++ actions ++ actionsR /\
+                                 actions0 = actions0' ++ actionsL}.
+Proof.
+  do 10 intro; intro Hsub; induction Hsub.
+  exists actions, []; repeat split.
+  rewrite app_nil_r; reflexivity.
+
+  destruct IHHsub as [actionsL [actionsR [Leq Req]]]; subst.
+  exists actionsL,(actionsR ++ [a]); split;[do 3 rewrite app_assoc|]; reflexivity.
+
+  destruct IHHsub as [actionsL [actionsR [Leq Req]]]; subst.
+  apply app_inv_head in Req; subst; apply app_inv_head in Leq.
+  cut (actions ++ [] = actions ++ actionsR).
+  intro H; apply app_inv_head in H; clear Leq;
+  exists actionsL,[]; split;[autorewrite with list; rewrite app_assoc|];reflexivity.
+  rewrite app_nil_r; auto.
+Qed.
+  
+End ActionTraces.
+End TraceClosures.
+
+Hint Constructors direct_clos_refl_trans clos_refl_trans_action clos_refl_trans_action_with_actions.
